LeanLgtm/Util.lean
@@ -8,13 +8,19 @@ open Lean Elab Command Term Meta Tactic
 
 register_simp_attr heapSimp
 
-partial def getList! (xs : Expr) : MetaM (List Expr) := do
-  match_expr xs with
-  | List.nil _ => return []
-  | List.cons _ x xs => do
-    let xs ← getList! xs
-    return x::xs
-  | _ => throwError "toLeanList: {xs} is not a list"
+-- partial def getList! (xs : Expr) : MetaM (List Expr) := do
+--   match_expr xs with
+--   | List.nil _ => return []
+--   | List.cons _ x xs => do
+--     let xs ← getList! xs
+--     return x::xs
+--   | _ => throwError "toLeanList: {xs} is not a list"
+
+partial def getList! (xs : Syntax) : (List Syntax) :=
+  match xs with
+  | `(List.nil) => []
+  | `(List.cons $x $xs) => x::getList! xs
+  | _ => panic! "getList!: {xs} is not a list"
 
 private def castToProp (e: Lean.Expr) : Lean.Elab.Tactic.TacticM (Option Q(Prop)) := do
   Qq.checkTypeQ (u := Lean.levelOne) e q(Prop)
@@ -24,6 +30,12 @@ def getGoalProp : Lean.Elab.Tactic.TacticM Q(Prop) := do
   match ← castToProp goal with
   | some qType => return qType
   | none => throwError "goal is not a proposition"
+
+
+def delabAll :=  (withOptions (fun _ => {}) $ PrettyPrinter.delab ·)
+
+def getGoalStxAll : Lean.Elab.Tactic.TacticM Syntax := do
+  delabAll $ <- getMainTarget
 
 
 
